LiveVerif/src/LiveVerifExamples/min.v
@@ -1,12 +1,15 @@
 (* -*- eval: (load-file "../LiveVerif/live_verif_setup.el"); -*- *)
 Require Import LiveVerif.LiveVerifLib. Load LiveVerif.
 
+(* TODO support functions that don't access any memory *)
+Definition dummy: mem -> Prop := emp True.
+
 #[export] Instance spec_of_u_min: fnspec :=                                     .**/
 
 uintptr_t u_min (uintptr_t a, uintptr_t b) /**#
   ghost_args := (R: mem -> Prop);
-  requires t m := sep (emp True) R m;
-  ensures t' m' retv := t' = t /\ sep (emp True) R m' /\
+  requires t m := sep dummy R m;
+  ensures t' m' retv := t' = t /\ sep dummy R m' /\
       (\[a] < \[b] /\ retv = a \/ \[b] <= \[a] /\ retv = b) #**/           /**.
 Derive u_min SuchThat (fun_correct! u_min) As u_min_ok.                         .**/
 {                                                                          /**. .**/
@@ -26,10 +29,10 @@ Import LiveSnippet.
 
 uintptr_t u_min3 (uintptr_t a, uintptr_t b, uintptr_t c) /**#
   ghost_args := (R: mem -> Prop);
-  requires t m := sep (emp True) R m;
+  requires t m := sep dummy R m;
   (* TODO make start_canceling work if just one R, or better, specialcase memoryless
      functions with m'=m in postcondition? *)
-  ensures t' m' retv := t' = t /\ sep (emp True) R m' /\
+  ensures t' m' retv := t' = t /\ sep dummy R m' /\
       \[retv] = Z.min \[a] (Z.min \[b] \[c]) #**/                          /**.
 Derive u_min3 SuchThat (fun_correct! u_min3) As u_min3_ok.                      .**/
 {                                                                          /**. .**/
