bedrock2/src/bedrock2/RecordPredicates.v
@@ -1,6 +1,8 @@
 Require Import Coq.ZArith.ZArith.
 Require Import coqutil.Word.Interface coqutil.Word.Bitwidth.
 Require Import coqutil.Map.Interface.
+Require Import coqutil.Tactics.RecordEta.
+Require Import coqutil.Tactics.Tactics.
 Require Import bedrock2.Map.Separation.
 Require Import bedrock2.SepLib.
 
@@ -24,16 +26,16 @@ Definition RepPredicate{width: Z}{BW: Bitwidth width}{word: word.word width}
   {mem: map.map word Byte.byte}(T: Type) := T -> word -> mem -> Prop.
 Existing Class RepPredicate.
 
-Global Hint Extern 1 (RepPredicate (uint_t ?nbits)) =>
+#[export] Hint Extern 1 (RepPredicate (uint_t ?nbits)) =>
   exact (uint nbits) : typeclass_instances.
 
-Global Hint Extern 1 (RepPredicate (array_t ?T ?n)) =>
+#[export] Hint Extern 1 (RepPredicate (array_t ?T ?n)) =>
   match constr:(_: RepPredicate T) with
   | ?elem => exact (array elem n)
   end
 : typeclass_instances.
 
-Global Hint Extern 1 (RepPredicate (@word.rep ?width ?word)) =>
+#[export] Hint Extern 1 (RepPredicate (@word.rep ?width ?word)) =>
   exact (@uintptr width _ word _) : typeclass_instances.
 
 Goal forall width (BW: Bitwidth width) (word: word width) (mem: map.map word Byte.byte)
@@ -67,14 +69,46 @@ Ltac create_predicate :=
              exact t'
   end.
 
+(* Given a match expression of the form
+   (match r with {| field1 := x1; ... fieldN := xn |} => body end),
+   returns a proof that this expression equals
+   body[field1 r/x1, ... fieldN r/xn] *)
+Ltac replace_match_by_projections_proof m :=
+  lazymatch m with
+  | (match ?d with _ => _ end) =>
+      let r := reconstruct_record d in
+      constr:(ltac:(replace d with r at 1 by (destruct d; reflexivity); reflexivity)
+               : m = _)
+  end.
+
+(* Given a goal of the form
+   PredicateSize (match r with {| field1 := x1; ... fieldN := xn |} => body end),
+   invoke typeclass search for
+   PredicateSize body[field1 r/x1, ... fieldN r/xn]
+   instead. *)
+Ltac tc_search_PredicateSize_of_projections_instead_of_match :=
+  lazymatch goal with
+  | |- PredicateSize ?m =>
+      let p := replace_match_by_projections_proof m in
+      lazymatch type of p with
+      | m = ?m' => lazymatch constr:(_ : PredicateSize m') with
+                   | ?s => exact s
+                   end
+      end
+  end.
+
+#[export] Hint Extern 20 (PredicateSize ?p) =>
+  let h := head p in unfold h; tc_search_PredicateSize_of_projections_instead_of_match
+: typeclass_instances.
+
 Module Examples_TODO_move.
 
 Definition MAC := array_t (uint_t 8) 6.
-Global Hint Extern 1 (RepPredicate MAC) =>
+#[export] Hint Extern 1 (RepPredicate MAC) =>
    exact (array (uint 8) 6) : typeclass_instances.
 
 Definition IPv4 := array_t (uint_t 8) 4.
-Global Hint Extern 1 (RepPredicate IPv4) =>
+#[export] Hint Extern 1 (RepPredicate IPv4) =>
   exact (array (uint 8) 4) : typeclass_instances.
 
 Definition ARPOperationRequest: Z := 1.
@@ -98,16 +132,31 @@ Record EthernetHeader_t := mkEthernetHeader {
   etherType: uint_t 16;
 }.
 
-Section WithMem.
+Record var_size_foo_t := {
+  foo_size: uint_t 32;
+  foo_payload: array_t (uint_t 8) foo_size;
+}.
 
+Section WithMem.
+  Local Open Scope Z_scope.
   Context {width: Z} {BW: Bitwidth width} {word: word.word width} {word_ok: word.ok word}.
   Context {mem: map.map word Byte.byte} {mem_ok: map.ok mem}.
 
-  Global Instance ARPPacket: RepPredicate ARPPacket_t :=
+  Instance ARPPacket: RepPredicate ARPPacket_t :=
     ltac:(create_predicate).
 
-  Global Instance EthernetHeader: RepPredicate EthernetHeader_t :=
+  Goal forall p, (_ : PredicateSize (ARPPacket p)) = 28. intros. reflexivity. Abort.
+
+  Instance EthernetHeader: RepPredicate EthernetHeader_t :=
     ltac:(create_predicate).
+
+  Goal forall p, (_ : PredicateSize (EthernetHeader p)) = 14. intros. reflexivity. Abort.
+
+  Instance var_size_foo: RepPredicate var_size_foo_t :=
+    ltac:(create_predicate).
+
+  Goal forall p, (_ : PredicateSize (var_size_foo p)) = 4 + foo_size p * 1.
+  Proof. intros. reflexivity. Abort.
 
   (* not a Lemma because this kind of goal will be solved inline by sepcalls canceler *)
   Goal forall (bs: list (uint_t 8)) (R: mem -> Prop) a m (Rest: EthernetHeader_t -> Prop),
